proof/correctness/avx2/1024/MLKEM_Poly_avx2_vec.ec
@@ -4,7 +4,7 @@ from Jasmin require import JModel.
 from JazzEC require import Array400 Array256 Array160 Array128 Array64 Array32 Array16 Array8 Array4.
 from JazzEC require import WArray800 WArray512 WArray128 WArray64 WArray32 WArray16.
 require import AVX2_Ops.
-from JazzEC require import Jkem1024_avx2.
+from JazzEC require import Jkem_avx2.
 require import MLKEM_Poly_avx2_prevec MLKEM_avx2_auxlemmas MLKEMFCLib.
 import MLKEMFCLib1024.
 
@@ -738,7 +738,7 @@ qed.
 
 
 equiv veceq_poly_add2 :
-  Mvec.poly_add2 ~Jkem1024_avx2.M._poly_add2: ={rp, bp} ==> ={res}.
+  Mvec.poly_add2 ~Jkem_avx2.M._poly_add2: ={rp, bp} ==> ={res}.
 proof.
   proc.
   while (={rp, bp, i}).
@@ -749,7 +749,7 @@ qed.
 
 
 equiv veceq_poly_sub :
-  Mvec.poly_sub ~Jkem1024_avx2.M._poly_sub: ={rp, ap, bp} ==> ={res}.
+  Mvec.poly_sub ~Jkem_avx2.M._poly_sub: ={rp, ap, bp} ==> ={res}.
 proof.
   proc.
   while (={rp, ap, bp, i}).
@@ -759,7 +759,7 @@ proof.
 qed.
 
 equiv veceq_poly_csubq :
-  Mvec.poly_csubq ~Jkem1024_avx2.M._poly_csubq: ={rp} ==> ={res}.
+  Mvec.poly_csubq ~Jkem_avx2.M._poly_csubq: ={rp} ==> ={res}.
 proof.
   proc.
   while (={rp, i, qx16}).
@@ -771,7 +771,7 @@ qed.
 
 
 equiv veceq_red16x:
-  Mvec.red16x ~Jkem1024_avx2.M.__red16x: ={r, qx16, vx16} ==> ={res}.
+  Mvec.red16x ~Jkem_avx2.M.__red16x: ={r, qx16, vx16} ==> ={res}.
 proof.
   proc.
   inline *.
@@ -779,7 +779,7 @@ proof.
 qed.
 
 equiv veceq_poly_reduce:
-  Mvec.poly_reduce ~Jkem1024_avx2.M.__poly_reduce: ={rp} ==> ={res}.
+  Mvec.poly_reduce ~Jkem_avx2.M.__poly_reduce: ={rp} ==> ={res}.
 proof.
   proc.
   while(={rp, i, qx16, vx16}).
@@ -789,7 +789,7 @@ proof.
 qed.
 
 equiv veceq_fqmulx16:
-  Mvec.fqmulx16 ~Jkem1024_avx2.M.__fqmulx16: ={a, b, qx16, qinvx16} ==> ={res}.
+  Mvec.fqmulx16 ~Jkem_avx2.M.__fqmulx16: ={a, b, qx16, qinvx16} ==> ={res}.
 proof.
   proc.
   inline *.
@@ -797,7 +797,7 @@ proof.
 qed.
 
 equiv veceq_poly_frommont:
-  Mvec.poly_frommont ~Jkem1024_avx2.M._poly_frommont: ={rp} ==> ={res}.
+  Mvec.poly_frommont ~Jkem_avx2.M._poly_frommont: ={rp} ==> ={res}.
 proof.
   proc.
   while(={rp, i, qx16, qinvx16, dmontx16} /\ aux{1} = inc{2}).
@@ -809,28 +809,28 @@ qed.
 
 
 equiv veceq_shuffle8:
-  Mvec.shuffle8 ~Jkem1024_avx2.M.__shuffle8: ={a, b} ==> ={res}.
+  Mvec.shuffle8 ~Jkem_avx2.M.__shuffle8: ={a, b} ==> ={res}.
 proof.
   proc.
   inline *; wp; skip; auto => />.
 qed.
 
 equiv veceq_shuffle4:
-  Mvec.shuffle4 ~Jkem1024_avx2.M.__shuffle4: ={a, b} ==> ={res}.
+  Mvec.shuffle4 ~Jkem_avx2.M.__shuffle4: ={a, b} ==> ={res}.
 proof.
   proc.
   inline *; wp; skip; auto => />.
 qed.
 
 equiv veceq_shuffle2:
-  Mvec.shuffle2 ~Jkem1024_avx2.M.__shuffle2: ={a, b} ==> ={res}.
+  Mvec.shuffle2 ~Jkem_avx2.M.__shuffle2: ={a, b} ==> ={res}.
 proof.
   proc.
   inline *; wp; skip; auto => />.
 qed.
 
 equiv veceq_shuffle1:
-  Mvec.shuffle1 ~Jkem1024_avx2.M.__shuffle1: ={a, b} ==> ={res}.
+  Mvec.shuffle1 ~Jkem_avx2.M.__shuffle1: ={a, b} ==> ={res}.
 proof.
   proc.
   inline *; wp; skip; auto => />.
@@ -838,7 +838,7 @@ qed.
 
 
 equiv prevec_eq_poly_add2:
-  Mprevec.poly_add2 ~Jkem1024_avx2.M._poly_add2: ={rp, bp} ==> ={res}.
+  Mprevec.poly_add2 ~Jkem_avx2.M._poly_add2: ={rp, bp} ==> ={res}.
     transitivity Mvec.poly_add2 (={rp, bp} ==> ={res}) (={rp, bp} ==> ={res}).
 smt(). trivial.
 apply eq_poly_add2.
@@ -846,7 +846,7 @@ apply veceq_poly_add2.
 qed.
 
 equiv prevec_eq_poly_sub:
-  Mprevec.poly_sub ~Jkem1024_avx2.M._poly_sub: ={rp, ap, bp} ==> ={res}.
+  Mprevec.poly_sub ~Jkem_avx2.M._poly_sub: ={rp, ap, bp} ==> ={res}.
     transitivity Mvec.poly_sub (={rp, ap, bp} ==> ={res}) (={rp, ap, bp} ==> ={res}).
 smt(). trivial.
 apply eq_poly_sub.
@@ -854,7 +854,7 @@ apply veceq_poly_sub.
 qed.
 
 equiv prevec_eq_poly_csubq:
-  Mprevec.poly_csubq ~Jkem1024_avx2.M._poly_csubq: ={rp} ==> ={res}.
+  Mprevec.poly_csubq ~Jkem_avx2.M._poly_csubq: ={rp} ==> ={res}.
     transitivity Mvec.poly_csubq (={rp} ==> ={res}) (={rp} ==> ={res}).
 smt(). trivial.
 apply eq_poly_csubq.
@@ -864,7 +864,7 @@ qed.
 
 
 equiv prevec_eq_red16x:
-  Mprevec.red16x ~Jkem1024_avx2.M.__red16x: is16u16 r{1} r{2} /\ is16u16 qx16{1} qx16{2} /\ is16u16 vx16{1} vx16{2} ==> is16u16 res{1} res{2}.
+  Mprevec.red16x ~Jkem_avx2.M.__red16x: is16u16 r{1} r{2} /\ is16u16 qx16{1} qx16{2} /\ is16u16 vx16{1} vx16{2} ==> is16u16 res{1} res{2}.
   transitivity Mvec.red16x (is16u16 r{1} r{2} /\ is16u16 qx16{1} qx16{2} /\ is16u16 vx16{1} vx16{2} ==> is16u16 res{1} res{2})
                            (={r, qx16, vx16} ==> ={res}).
 smt(). trivial.
@@ -873,7 +873,7 @@ apply veceq_red16x.
 qed.
 
 equiv prevec_eq_poly_reduce:
-  Mprevec.poly_reduce ~Jkem1024_avx2.M.__poly_reduce: ={rp} ==> ={res}.
+  Mprevec.poly_reduce ~Jkem_avx2.M.__poly_reduce: ={rp} ==> ={res}.
     transitivity Mvec.poly_reduce (={rp} ==> ={res}) (={rp} ==> ={res}).
 smt(). trivial.
 apply eq_poly_reduce.
@@ -881,7 +881,7 @@ apply veceq_poly_reduce.
 qed.
 
 equiv prevec_eq_fqmulx16:
-  Mprevec.fqmulx16 ~Jkem1024_avx2.M.__fqmulx16: is16u16 a{1} a{2} /\ is16u16 b{1} b{2} /\ is16u16 qx16{1} qx16{2} /\ is16u16 qinvx16{1} qinvx16{2} ==> is16u16 res{1} res{2}.
+  Mprevec.fqmulx16 ~Jkem_avx2.M.__fqmulx16: is16u16 a{1} a{2} /\ is16u16 b{1} b{2} /\ is16u16 qx16{1} qx16{2} /\ is16u16 qinvx16{1} qinvx16{2} ==> is16u16 res{1} res{2}.
     transitivity Mvec.fqmulx16 (is16u16 a{1} a{2} /\ is16u16 b{1} b{2} /\ is16u16 qx16{1} qx16{2} /\ is16u16 qinvx16{1} qinvx16{2} ==> is16u16 res{1} res{2})
                                (={a, b, qx16, qinvx16} ==> ={res}).
 smt(). trivial.
@@ -890,7 +890,7 @@ apply veceq_fqmulx16.
 qed.
 
 equiv prevec_eq_poly_frommont:
-  Mprevec.poly_frommont ~Jkem1024_avx2.M._poly_frommont: ={rp} ==> ={res}.
+  Mprevec.poly_frommont ~Jkem_avx2.M._poly_frommont: ={rp} ==> ={res}.
     transitivity Mvec.poly_frommont (={rp} ==> ={res}) (={rp} ==> ={res}).
 smt(). trivial.
 apply eq_poly_frommont.
@@ -899,7 +899,7 @@ qed.
 
 
 equiv prevec_eq_shuffle8:
-  Mprevec.shuffle8 ~Jkem1024_avx2.M.__shuffle8: is16u16 a{1} a{2} /\ is16u16 b{1} b{2} ==>
+  Mprevec.shuffle8 ~Jkem_avx2.M.__shuffle8: is16u16 a{1} a{2} /\ is16u16 b{1} b{2} ==>
                                     is16u16 res{1}.`1 res{2}.`1 /\
                                     is16u16 res{1}.`2 res{2}.`2.
 proof.
@@ -913,13 +913,13 @@ proof.
 qed.
 
 equiv prevec_eq_shuffle8_sym :
-  Jkem1024_avx2.M.__shuffle8 ~ Mprevec.shuffle8 : is16u16 a{2} a{1} /\ is16u16 b{2} b{1} ==>
+  Jkem_avx2.M.__shuffle8 ~ Mprevec.shuffle8 : is16u16 a{2} a{1} /\ is16u16 b{2} b{1} ==>
                                     is16u16 res{2}.`1 res{1}.`1 /\
                                     is16u16 res{2}.`2 res{1}.`2.
 symmetry. conseq prevec_eq_shuffle8 => />. qed.
 
 equiv prevec_eq_shuffle4:
-  Mprevec.shuffle4 ~Jkem1024_avx2.M.__shuffle4: is16u16 a{1} a{2} /\ is16u16 b{1} b{2} ==>
+  Mprevec.shuffle4 ~Jkem_avx2.M.__shuffle4: is16u16 a{1} a{2} /\ is16u16 b{1} b{2} ==>
                                     is16u16 res{1}.`1 res{2}.`1 /\
                                     is16u16 res{1}.`2 res{2}.`2.
 proof.
@@ -933,13 +933,13 @@ proof.
 qed.
 
 equiv prevec_eq_shuffle4_sym:
-  Jkem1024_avx2.M.__shuffle4 ~ Mprevec.shuffle4: is16u16 a{2} a{1} /\ is16u16 b{2} b{1} ==>
+  Jkem_avx2.M.__shuffle4 ~ Mprevec.shuffle4: is16u16 a{2} a{1} /\ is16u16 b{2} b{1} ==>
                                     is16u16 res{2}.`1 res{1}.`1 /\
                                     is16u16 res{2}.`2 res{1}.`2.
 symmetry. conseq prevec_eq_shuffle4 => />. qed.
 
 equiv prevec_eq_shuffle2:
-  Mprevec.shuffle2 ~Jkem1024_avx2.M.__shuffle2: is16u16 a{1} a{2} /\ is16u16 b{1} b{2} ==>
+  Mprevec.shuffle2 ~Jkem_avx2.M.__shuffle2: is16u16 a{1} a{2} /\ is16u16 b{1} b{2} ==>
                                     is16u16 res{1}.`1 res{2}.`1 /\
                                     is16u16 res{1}.`2 res{2}.`2.
 proof.
@@ -953,13 +953,13 @@ proof.
 qed.
 
 equiv prevec_eq_shuffle2_sym:
-  Jkem1024_avx2.M.__shuffle2 ~ Mprevec.shuffle2 : is16u16 a{2} a{1} /\ is16u16 b{2} b{1} ==>
+  Jkem_avx2.M.__shuffle2 ~ Mprevec.shuffle2 : is16u16 a{2} a{1} /\ is16u16 b{2} b{1} ==>
                                     is16u16 res{2}.`1 res{1}.`1 /\
                                     is16u16 res{2}.`2 res{1}.`2.
 symmetry. conseq prevec_eq_shuffle2 => />. qed.
 
 equiv prevec_eq_shuffle1:
-  Mprevec.shuffle1 ~Jkem1024_avx2.M.__shuffle1: is16u16 a{1} a{2} /\ is16u16 b{1} b{2} ==>
+  Mprevec.shuffle1 ~Jkem_avx2.M.__shuffle1: is16u16 a{1} a{2} /\ is16u16 b{1} b{2} ==>
                                     is16u16 res{1}.`1 res{2}.`1 /\
                                     is16u16 res{1}.`2 res{2}.`2.
 proof.
@@ -973,7 +973,7 @@ proof.
 qed.
 
 equiv prevec_eq_shuffle1_sym:
-  Jkem1024_avx2.M.__shuffle1 ~ Mprevec.shuffle1 : is16u16 a{2} a{1} /\ is16u16 b{2} b{1} ==>
+  Jkem_avx2.M.__shuffle1 ~ Mprevec.shuffle1 : is16u16 a{2} a{1} /\ is16u16 b{2} b{1} ==>
                                     is16u16 res{2}.`1 res{1}.`1 /\
                                     is16u16 res{2}.`2 res{1}.`2.
 symmetry. conseq prevec_eq_shuffle1 => />. qed.
@@ -986,7 +986,7 @@ lemma list_arr16 (x:'a Array16.t):
 rewrite /to_list /mkseq -iotaredE => />. qed.
 
 lemma avx2_shuffle8_corr_h (_a _b : t16u16) :
-      hoare[ Jkem1024_avx2.M.__shuffle8 :
+      hoare[ Jkem_avx2.M.__shuffle8 :
              is16u16 _a a /\ is16u16 _b b
              ==>
              is16u16 (NTT_Avx2.shuf8 _a _b).`1 res.`1 /\
@@ -996,7 +996,7 @@ auto => /> &1 -> ->. exists ((_a,_b)) => />.
 auto => /> &1 &2 -> -> -> ->. rewrite /is16u16 !list_arr16 //. qed.
 
 lemma avx2_shuffle8_corr (_a _b : t16u16) :
-      phoare[ Jkem1024_avx2.M.__shuffle8 :
+      phoare[ Jkem_avx2.M.__shuffle8 :
              is16u16 _a a /\ is16u16 _b b
              ==>
              is16u16 (NTT_Avx2.shuf8 _a _b).`1 res.`1 /\
@@ -1004,7 +1004,7 @@ lemma avx2_shuffle8_corr (_a _b : t16u16) :
 conseq __shuffle8_ll (avx2_shuffle8_corr_h _a _b) => />. qed.
 
 lemma avx2_shuffle4_corr_h (_a _b : t16u16) :
-      hoare[ Jkem1024_avx2.M.__shuffle4 :
+      hoare[ Jkem_avx2.M.__shuffle4 :
              is16u16 _a a /\ is16u16 _b b
              ==>
              is16u16 (NTT_Avx2.shuf4 _a _b).`1 res.`1 /\
@@ -1014,7 +1014,7 @@ auto => /> &1 -> ->. exists ((_a,_b)) => />.
 auto => /> &1 &2 -> -> -> ->. rewrite /is16u16 !list_arr16 //. qed.
 
 lemma avx2_shuffle4_corr (_a _b : t16u16) :
-      phoare[ Jkem1024_avx2.M.__shuffle4 :
+      phoare[ Jkem_avx2.M.__shuffle4 :
              is16u16 _a a /\ is16u16 _b b
              ==>
              is16u16 (NTT_Avx2.shuf4 _a _b).`1 res.`1 /\
@@ -1022,7 +1022,7 @@ lemma avx2_shuffle4_corr (_a _b : t16u16) :
 conseq __shuffle4_ll (avx2_shuffle4_corr_h _a _b) => />. qed.
 
 lemma avx2_shuffle2_corr_h (_a _b : t16u16) :
-      hoare[ Jkem1024_avx2.M.__shuffle2 :
+      hoare[ Jkem_avx2.M.__shuffle2 :
              is16u16 _a a /\ is16u16 _b b
              ==>
              is16u16 (NTT_Avx2.shuf2 _a _b).`1 res.`1 /\
@@ -1032,7 +1032,7 @@ auto => /> &1 -> ->. exists ((_a,_b)) => />.
 auto => /> &1 &2 -> -> -> ->. rewrite /is16u16 !list_arr16 //. qed.
 
 lemma avx2_shuffle2_corr (_a _b : t16u16) :
-      phoare[ Jkem1024_avx2.M.__shuffle2 :
+      phoare[ Jkem_avx2.M.__shuffle2 :
              is16u16 _a a /\ is16u16 _b b
              ==>
              is16u16 (NTT_Avx2.shuf2 _a _b).`1 res.`1 /\
@@ -1040,7 +1040,7 @@ lemma avx2_shuffle2_corr (_a _b : t16u16) :
 conseq __shuffle2_ll (avx2_shuffle2_corr_h _a _b) => />. qed.
 
 lemma avx2_shuffle1_corr_h (_a _b : t16u16) :
-      hoare[ Jkem1024_avx2.M.__shuffle1 :
+      hoare[ Jkem_avx2.M.__shuffle1 :
              is16u16 _a a /\ is16u16 _b b
              ==>
              is16u16 (NTT_Avx2.shuf1 _a _b).`1 res.`1 /\
@@ -1050,7 +1050,7 @@ auto => /> &1 -> ->. exists ((_a,_b)) => />.
 auto => /> &1 &2 -> -> -> ->. rewrite /is16u16 !list_arr16 //. qed.
 
 lemma avx2_shuffle1_corr (_a _b : t16u16) :
-      phoare[ Jkem1024_avx2.M.__shuffle1 :
+      phoare[ Jkem_avx2.M.__shuffle1 :
              is16u16 _a a /\ is16u16 _b b
              ==>
              is16u16 (NTT_Avx2.shuf1 _a _b).`1 res.`1 /\
