proof/correctness/avx2/768/MLKEM_Poly_avx2_proof.ec
@@ -9,7 +9,7 @@ require import AVX2_Ops MLKEM_Poly_avx2_prevec NTT_avx2 Fq_avx2 MLKEM_avx2_auxle
 require import Fq NTT_Fq MLKEMFCLib.
 import MLKEMFCLib768.
 
-from JazzEC require import Jkem768_avx2.
+from JazzEC require import Jkem_avx2.
 
 from Spec require import GFq Rq Serialization VecMat Correctness768.
 
@@ -233,7 +233,7 @@ lemma poly_csubq_corr_h ap :
              pos_bound256_cxq res 0 256 1 ].
 proof.
   proc.
-  while (ap = lift_array256 rp /\ pos_bound256_cxq rp 0 256 2 /\ pos_bound256_cxq rp 0 (16*i) 1 /\ 0 <= i <= 16 /\ forall k, 0 <= k < 16 => _qx16.[k] = Jkem768_avx2.jqx16.[k]).
+  while (ap = lift_array256 rp /\ pos_bound256_cxq rp 0 256 2 /\ pos_bound256_cxq rp 0 (16*i) 1 /\ 0 <= i <= 16 /\ forall k, 0 <= k < 16 => _qx16.[k] = Jkem_avx2.jqx16.[k]).
   seq 3 : (#pre /\ forall k, 0 <= k < 16 => _r.[k] = rp.[16 * i + k] - _qx16.[k]).
   inline Ops.iVPSUB_16u16.
   wp. skip. simplify.
@@ -323,7 +323,7 @@ proof.
   (****)
   rewrite to_sintN => //=.
   rewrite (_qx16_def (x%% 16))  => //=.
-  rewrite /(Jkem768_avx2.jqx16).
+  rewrite /(Jkem_avx2.jqx16).
   rewrite get_of_list => />.
   do rewrite fun_if.
   rewrite of_sintK /= /smod.
@@ -331,7 +331,7 @@ proof.
   simplify.
   smt().
   rewrite _qx16_def => //=.
-  rewrite /(Jkem768_avx2.jqx16).
+  rewrite /(Jkem_avx2.jqx16).
   rewrite get_of_list => />.
   do rewrite fun_if.
   rewrite of_sintK /= /smod /=.
@@ -342,13 +342,13 @@ proof.
   
   rewrite to_sintN => //=.
   rewrite _qx16_def => //=.
-  rewrite /(Jkem768_avx2.jqx16).
+  rewrite /(Jkem_avx2.jqx16).
   rewrite get_of_list => />.
   do rewrite fun_if.
   rewrite of_sintK /= /smod.
   smt().
   rewrite _qx16_def => //=.
-  rewrite /(Jkem768_avx2.jqx16).
+  rewrite /(Jkem_avx2.jqx16).
   rewrite get_of_list => />.
   do rewrite fun_if.
   rewrite of_sintK /= /smod.
@@ -358,7 +358,7 @@ proof.
   rewrite _qx16_def => //=.
   rewrite (_: rp{hr}.[16 * i{hr} + x %% 16] = rp{hr}.[x]).
     by move : x_i x_mb => /#.
-  rewrite /(Jkem768_avx2.jqx16).
+  rewrite /(Jkem_avx2.jqx16).
   rewrite get_of_list => />.
   do rewrite fun_if.
   rewrite incoeffD. ring.
@@ -424,7 +424,7 @@ proof.
   rewrite W16.sltE.
   rewrite to_sintB_small.
   rewrite _qx16_def => //=.
-  rewrite /(Jkem768_avx2.jqx16).
+  rewrite /(Jkem_avx2.jqx16).
   rewrite get_of_list => />.
   do rewrite fun_if.
   do rewrite of_sintK.
@@ -435,7 +435,7 @@ proof.
   rewrite idx_bounds /= qE /=.
   smt().
   rewrite _qx16_def => //=.
-  rewrite /(Jkem768_avx2.jqx16).
+  rewrite /(Jkem_avx2.jqx16).
   rewrite get_of_list => />.
   do rewrite fun_if.
   do rewrite of_sintK.
@@ -446,7 +446,7 @@ proof.
   rewrite to_sintD_small => />.
   rewrite to_sintN => />.
   rewrite _qx16_def => //=.
-  rewrite /(Jkem768_avx2.jqx16).
+  rewrite /(Jkem_avx2.jqx16).
   rewrite get_of_list => />.
   do rewrite fun_if.
   do rewrite of_sintK => />.
@@ -459,7 +459,7 @@ proof.
   rewrite _r_def => //.
   rewrite sltE.
   rewrite _qx16_def => //=.
-  rewrite /(Jkem768_avx2.jqx16).
+  rewrite /(Jkem_avx2.jqx16).
   rewrite get_of_list => />.
   rewrite to_sintB_small.
   do rewrite fun_if.
@@ -485,7 +485,7 @@ proof.
   rewrite _r_def => //.
   rewrite sltE.
   rewrite _qx16_def => //=.
-  rewrite /(Jkem768_avx2.jqx16).
+  rewrite /(Jkem_avx2.jqx16).
   rewrite get_of_list => />.
   rewrite to_sintB_small.
   do rewrite fun_if.
@@ -508,7 +508,7 @@ proof.
   smt().
 
   rewrite _qx16_def => //=.
-  rewrite /(Jkem768_avx2.jqx16).
+  rewrite /(Jkem_avx2.jqx16).
   rewrite get_of_list => />.
   do rewrite fun_if.
   rewrite to_sintN /=.
@@ -555,7 +555,7 @@ proof.
   move : _r_ub.
   rewrite sltE.
   rewrite _qx16_def => //=.
-  rewrite /(Jkem768_avx2.jqx16).
+  rewrite /(Jkem_avx2.jqx16).
   rewrite get_of_list => />.
   rewrite to_sintB_small.
   do rewrite fun_if.
@@ -582,7 +582,7 @@ proof.
   move : _r_lb.
   rewrite sltE.
   rewrite _qx16_def => //=.
-  rewrite /(Jkem768_avx2.jqx16).
+  rewrite /(Jkem_avx2.jqx16).
   rewrite get_of_list => />.
   rewrite to_sintB_small.
   do rewrite fun_if.
@@ -602,7 +602,7 @@ proof.
   rewrite to_sintD_small => />.
   rewrite to_sintN => />.
   rewrite _qx16_def => //=.
-  rewrite /(Jkem768_avx2.jqx16).
+  rewrite /(Jkem_avx2.jqx16).
   rewrite get_of_list => />.
   do rewrite fun_if.
   rewrite of_sintK => />.
@@ -614,7 +614,7 @@ proof.
   move : _r_lb.
   rewrite sltE.
   rewrite _qx16_def => //=.
-  rewrite /(Jkem768_avx2.jqx16).
+  rewrite /(Jkem_avx2.jqx16).
   rewrite get_of_list => />.
   rewrite to_sintB_small.
   do rewrite fun_if.
@@ -633,7 +633,7 @@ proof.
   move : _r_lb.
   rewrite sltE.
   rewrite _qx16_def => //=.
-  rewrite /(Jkem768_avx2.jqx16).
+  rewrite /(Jkem_avx2.jqx16).
   rewrite get_of_list => />.
   rewrite to_sintB_small.
   do rewrite fun_if.
@@ -644,7 +644,7 @@ proof.
 
   move : _sr_lb rp_qx16_lb.
   rewrite _qx16_def => //=.
-  rewrite /(Jkem768_avx2.jqx16).
+  rewrite /(Jkem_avx2.jqx16).
   rewrite get_of_list => />.
   rewrite to_sintB_small.
   do rewrite fun_if.
@@ -661,7 +661,7 @@ proof.
   
   rewrite qE.
   rewrite _qx16_def => //=.
-  rewrite /(Jkem768_avx2.jqx16).
+  rewrite /(Jkem_avx2.jqx16).
   rewrite get_of_list => />.
   do rewrite fun_if.
   rewrite to_sintN of_sintK => />.
@@ -670,7 +670,7 @@ proof.
   move : _r_lb.
   rewrite sltE.
   rewrite _qx16_def => //=.
-  rewrite /(Jkem768_avx2.jqx16).
+  rewrite /(Jkem_avx2.jqx16).
   rewrite get_of_list => />.
   rewrite to_sintB_small.
   do rewrite fun_if.
@@ -682,7 +682,7 @@ proof.
   move => rp_q_lb_neg.
   move : _sr_lb.
   rewrite _qx16_def => //=.
-  rewrite /(Jkem768_avx2.jqx16).
+  rewrite /(Jkem_avx2.jqx16).
   rewrite get_of_list => />.
   rewrite to_sintB_small.
   do rewrite fun_if.
@@ -755,8 +755,8 @@ proof.
   while (0 <= i <= 16 /\
          (forall k, 0 <= k < 256 => ap.[k] = incoeff (to_sint rp.[k])) /\
          (forall k, 0 <= k < 16 * i => bpos16 rp.[k] (2*q)) /\
-         (forall k, 0 <= k < 16 => qx16.[k] = Jkem768_avx2.jqx16.[k]) /\
-         (forall k, 0 <= k < 16 => vx16.[k] = Jkem768_avx2.jvx16.[k])); last first.
+         (forall k, 0 <= k < 16 => qx16.[k] = Jkem_avx2.jqx16.[k]) /\
+         (forall k, 0 <= k < 16 => vx16.[k] = Jkem_avx2.jvx16.[k])); last first.
   wp. skip.
   move => &hr ap_def />.
   do split.
@@ -894,7 +894,7 @@ proof.
   rewrite (_: (2 * k + 1) %% 2 = 1).
     by smt().
   rewrite pack2_bits8.
-  rewrite /(Jkem768_avx2.jdmontx16) => />.
+  rewrite /(Jkem_avx2.jdmontx16) => />.
   rewrite initiE => />. move : k_lb k_ub => /#.
   smt().
   
@@ -914,7 +914,7 @@ proof.
   rewrite (_: (2 * k + 1) %% 2 = 1).
     by smt().
   rewrite pack2_bits8.
-  rewrite /(Jkem768_avx2.jqx16) => />.
+  rewrite /(Jkem_avx2.jqx16) => />.
   rewrite initiE => />. move : k_lb k_ub => /#.
   smt().
   
